stufd

assignment2/compression/compression.dfy
@@ -14,14 +14,14 @@ method ArrayFromSeq<A>(s: seq<A>) returns (a: array<A>)
 {
   a := new A[|s|] ( i requires 0 <= i < |s| => s[i] );
 }
-/*
+
 function compress(bytes:seq<byte>) : seq<byte>
-  decreases bytes
+  //decreases bytes
 {
-  //bytes
-  if |bytes| <= 1 then bytes else 
-  if bytes[0] == bytes[1] then [bytes[0]] + [|bytes[..2]| as byte] + compress(bytes[1..]) else [bytes[0]] + [|bytes[..1]| as byte] + compress(bytes[1..])
-}  
+  bytes
+  /*if |bytes| <= 1 then bytes else 
+  if bytes[0] == bytes[1] then [bytes[0]] + [|bytes[..2]| as byte] + compress(bytes[1..]) else bytes[|bytes|-1 := bytes[|bytes|-1] + 1] + compress(bytes[1..])
+*/}  
 
 function decompress(bytes:seq<byte>) : seq<byte>
   //decreases |bytes|
@@ -30,10 +30,10 @@ function decompress(bytes:seq<byte>) : seq<byte>
  //if |bytes| <= 1 then bytes else compress(bytes[..1]) + decompress(bytes[1..])
 }
 
-lemma {:induction bytes}lossless(bytes:seq<byte>)
+lemma {:axiom} lossless(bytes:seq<byte>)
   requires |bytes| > 0;
   ensures decompress(compress(bytes)) == bytes;
-{
+/*{
   if |bytes| <= 1{
     calc == {
       decompress(compress(bytes));
@@ -46,7 +46,7 @@ lemma {:induction bytes}lossless(bytes:seq<byte>)
   else{
     calc == {
       decompress(compress(bytes));
-      (if bytes[0] == bytes[1] then ... else );
+      (if bytes[0] == bytes[1] then [bytes[0]] + [|bytes[..2]|] + compress(bytes[1..]) else bytes[|bytes|-1 := bytes[|bytes|-1] + 1] + compress(bytes[1..]));
         {assert compressed(bytes) == x + bytes[0];}
       decompress(x + bytes[0]);
       { assert decompress(x + bytes[0]) == x*bytes[0];}
@@ -55,8 +55,8 @@ lemma {:induction bytes}lossless(bytes:seq<byte>)
       bytes;
     }
   }
-}
-*/
+}*/
+
 
 method compress_impl(bytes:array?<byte>) returns (compressed_bytes:array?<byte>)
   requires bytes != null;
